lvaluestreams, contraction proof of concept. WIP
probably incorrect expansion attempt

etch4/Etch/Stream3.lean
@@ -1,25 +1,55 @@
-import Lean
+import Init.Data.List.Basic
 
 import Mathlib.Data.Nat.Basic
 import Mathlib.Data.Option.Basic
+import Mathlib.Data.Finset.Card
 import Mathlib.Tactic.LibrarySearch
+import Mathlib.Tactic.Linarith
 
 import Etch.C
 import Etch.Basic
 --import Init.WFTactics
 
+namespace List
+-- Same as List.Mem, except this lives in Type
+inductive Here (a : α) : List α → Type
+| head (as : List α) : Here a (a::as)
+| tail (b : α) {as : List α} : Here a as → Here a (b::as)
+
+@[reducible]
+def eraseHere : (xs : List α) → Here x xs → List α
+| _ :: xs, .head _ => xs
+| _, .tail b tail => b :: eraseHere _ tail
+
+#eval [1,2].eraseHere $ .tail _ (.head _)
+
+example : 1 ∈ [2,1,3] := by decide
+
+class Find (x : α) (xs : List α) where here : Here x xs
+instance Find.tail [Find x xs] : Find x (y :: xs) where here := .tail _ Find.here
+instance Find.head : Find x (x :: xs) where here := .head _
+
+def remove (x : α) (xs : List α) [Find x xs] : List α := xs.eraseHere (x := x) Find.here
+#eval remove 1 [3,3,3,1,2,3,3,1,3,4,5,55,5,6,2]
+
+end List
+
 namespace Etch
 
 variable (A : Type) [Inhabited A]
 
-@[reducible] abbrev Var := String
-def Var.toString : Var → String := id
+structure Shape where
+  val : List A
+  nodup : List.Nodup val
 
 inductive EType : Type
-| attr : A → EType -- user-selected attribute types
 | bool -- internal boolean type
 | int  -- internal int type
-| k : A → EType -- universal semiring type
+| attr : A → EType -- user-selected attribute types
+| k    : A → EType -- universal semiring type
+
+@[reducible] abbrev Var (A) (_ : EType A) := String
+def Var.toString : Var A i → String := id
 
 instance : Coe A (EType A) where coe := EType.attr
 
@@ -37,20 +67,20 @@ structure Op (out : EType A) : Type where
   arity : ℕ
   params : Fin arity → EType A
   name : String
-attribute [reducible] Op.params
-attribute [reducible] Op.arity
+attribute [reducible] Op.params Op.arity
 
 variable {A}
 -- an operator parametrized by its output type
 @[simps, reducible] def monotypicOp {n} (params : Fin n → EType A) (s : String) : Op A t := ⟨ _, params, s!"{t.toTag}_{s}" ⟩
 
 section Op
-variable {i : A}
-@[reducible] def Op.lt : Op A .bool := monotypicOp ![i, i] "lt"
-@[reducible] def Op.le : Op A .bool := monotypicOp ![i, i] "le"
+variable {i : A} {t : EType A}
+@[reducible] def Op.lt : Op A .bool := monotypicOp ![t, t] "lt"
+@[reducible] def Op.neg : Op A .bool := monotypicOp ![.bool] "neg"
+@[reducible] def Op.le : Op A .bool := monotypicOp ![t, t] "le"
 @[reducible] def Op.max : Op A i := monotypicOp ![i, i] "max"
-@[reducible] def Op.eq : Op A .bool := monotypicOp ![i, i] "eq"
-@[reducible] def Op.min : Op A i := monotypicOp ![i, i] "min"
+@[reducible] def Op.eq : Op A .bool := monotypicOp ![t, t] "eq"
+@[reducible] def Op.min {t : EType A} : Op A i := monotypicOp ![t, t] "min"
 @[reducible] def Op.true : Op A .bool := ⟨ _, ![], "true" ⟩
 @[reducible] def Op.false : Op A .bool := ⟨ _, ![], "false" ⟩
 @[reducible] def Op.and : Op A .bool := monotypicOp ![.bool, .bool] "and"
@@ -59,7 +89,8 @@ variable {i : A}
 @[reducible] def Op.one : Op A (.k i) := ⟨ _, ![], "one" ⟩
 @[reducible] def Op.int_one : Op A .int := ⟨ _, ![], "one" ⟩
 @[reducible] def Op.add : Op A (.k i) := monotypicOp ![.k i, .k i] "add"
-@[reducible] def Op.int_add : Op A .int := monotypicOp ![.int, .int] "add"
+@[reducible] def Op.int_add : Op A .int := monotypicOp ![.int, .int] "add" -- sic
+@[reducible] def Op.int_sub : Op A .int := monotypicOp ![.int, .int] "sub"
 @[reducible] def Op.mul {i j k : A} : Op A (.k i) := monotypicOp ![.k j, .k k] "mul"
 -- parametrized by input and output type. semantic no-op
 @[reducible] def Op.to (i i' : EType A) : Op A i' := ⟨ _, ![i], s!"{i.toTag}_to_{i'.toTag}" ⟩
@@ -67,40 +98,41 @@ end Op
 
 variable (A)
 inductive E : EType A → Type
-| var (t : EType A) (v : Var) : E t
+| var {t : EType A} (v : Var A t) : E t
 | call {t} (op : Op A t) (args : (i : Fin op.arity) → E (op.params i)) : E t
-| access (t : EType A) (v : Var) (ind : E .int) : E t
+| access {t : EType A} (v : Var A t) (ind : E .int) : E t
 
 def E.compile : E A t → Expr
-| var _ v => Expr.var v.toString
+| var v => Expr.var v.toString
 | call op args => Expr.call (t.toTag ++ op.name) $ List.ofFn λ i => E.compile (args i)
-| access _ base i => Expr.index (Expr.var base.toString) [i.compile]
+| access base i => Expr.index (Expr.var base.toString) [i.compile]
 
-def Var.expr : Var → E A i := .var _
 
-inductive LVal
-| local : Var → LVal
-| mem   : Var → E A .int → LVal
+def Var.expr {A} {t : EType A} : Var A t → E A t := .var
+instance : Coe (Var A t) (E A t) := ⟨ Var.expr ⟩
 
-def LVal.expr : LVal A → E A t
-| .local v => .var _ v
-| .mem var i => .access _ var i
+inductive LVal (t : EType A)
+| local : Var A t → LVal t
+| mem   : Var A t → E A .int → LVal t
+
+def LVal.expr : LVal A t → E A t
+| .local v => .var v
+| .mem var i => .access var i
 
 inductive P : Type
 | skip
 | seq   : P → P → P
-| load  : E A .int → Var → P
+--| load  {i : EType A} : E A .int → Var A i → P
 | branch: E A .bool → P → P → P
 | while : E A .bool → P → P
-| store : LVal A → E A t → P
-| let : Var → E A t → P → P
---| store_var {t} : Var → E A t → P
---| store_mem {i : A} : Var → E A .int → E A (.k i) → P
+| store : LVal A t → E A t → P
+| let : Var A t → E A t → P → P
 
 instance : Inhabited (P A) where default := .skip
 
 infixr:10 " ;; " => P.seq
 def P.if1 {A} : E A .bool → P A → P A := fun c t ↦ P.branch c t P.skip
+
 
 structure Level {A} (i : A) : Type where
   skip  : E A i → E A .bool → P A
@@ -120,6 +152,10 @@ infixr:40 " >= " => λ a b => E.call Op.le ![b, a]
 instance : Zero (E A (.k i)) := ⟨ E.call Op.zero ![] ⟩
 instance : One (E A (.k i)) := ⟨ E.call Op.one ![] ⟩
 instance : One (E A .int) := ⟨ E.call Op.int_one ![] ⟩
+instance : Add (E A .int) := ⟨ λ a b => E.call .int_add ![a, b] ⟩
+instance : Sub (E A .int) := ⟨ λ a b => E.call .int_sub ![a, b] ⟩
+
+def LVal.incr : LVal A .int → P A := fun l ↦ .store l (l.expr + (1 : E A .int))
 
 infixr:min "$!" => E.call
 
@@ -128,19 +164,19 @@ def E.or : E A .bool → E A .bool → E A .bool := fun a b ↦ E.call Op.and ![
 
 variable {A}
 
-def Var.subst (v : Var) (val : Var) : Var → Var
-| v' => if v = v' then val else v'
+def Var.subst (v : Var A t) (val : Var A t) : ∀ {s : EType A}, Var A s → Var A s
+| _, v' => if v = v' then val else v'
 
-def E.subst (v : Var) (val : Var) : ∀ {t}, E A t → E A t := sorry
+def E.subst (v : Var A t) (val : Var A t) : {t : EType A} → E A t → E A t := sorry
 
-def LVal.subst (v : Var) (val : Var) : LVal A → LVal A
-| .local l => .local $ l.subst v val
-| mem l i => .mem (l.subst v val) (i.subst v val)
+def LVal.subst (v : Var A t) (val : Var A t) : ∀ {t}, LVal A t → LVal A t
+| _, .local l => .local $ l.subst v val
+| _, mem l i => .mem (l.subst v val) (i.subst v val)
 
-def P.subst (v : Var) (val : Var) : P A → P A
+def P.subst (v : Var A t) (val : Var A t) : P A → P A
 | skip => .skip
 | seq a b => .seq (subst v val a) (subst v val b)
-| load l r => .load (l.subst v val) (r.subst v val)
+--| load l r => .load (l.subst (t := .int) v val) (r.subst v val)
 | branch c t f => .branch (c.subst v val) (t.subst v val) (f.subst v val)
 | .while c t => .while (c.subst v val) (t.subst v val)
 | .let v' e b => .let v' (e.subst v val) (if v = v' then b else b.subst v val)
@@ -150,7 +186,7 @@ abbrev M := StateM ℕ
 def M.run' : ℕ → M α → α := fun n c ↦ Prod.fst (StateT.run c n).run
 def M.run : M α → α := fun c ↦ Prod.fst (StateT.run c 0).run
 def freshNat : M ℕ := do let n ← get; modify (. + 1); pure n
-def freshen (v : Var) : M Var := do pure s!"{v}_{(← freshNat)}"
+def freshen (v : Var A t) : M (Var A t) := do pure s!"{v}_{(← freshNat)}"
 
 --def P.compile : P A → Stmt
 --| seq a b            => Stmt.seq a.compile b.compile
@@ -168,7 +204,7 @@ def P.compile : P A → M Stmt
 | skip               => pure Stmt.noop
 | store (.local l) r => pure $ Stmt.store (Expr.var l.toString) r.compile
 | store (.mem v i) r => pure $ Stmt.store (Expr.index (Expr.var v.toString) [i.compile]) r.compile
-| load addr v        => pure $ Stmt.store (Expr.var v.toString) (Expr.index (addr.compile) [0])
+--| load addr v        => pure $ Stmt.store (Expr.var v.toString) (Expr.index (addr.compile) [0])
 | .let v e b         => do let v' ← freshen v; Stmt.seq (Stmt.store (.var v') e.compile) <$> b.compile
 
 variable {i : A}
@@ -178,37 +214,127 @@ def Level.mul (a : Level i) (b : Level i) : Level i where
   valid := .and $! ![a.valid, b.valid]
   skip  i r := a.skip i r;; b.skip i r
 
-def Level.range (ctr size inds : Var) : Level i :=
-  let ind := .access i inds (.var .int ctr)
+def Level.range (ctr size : Var A .int) (inds : Var A (.attr i)) : Level i :=
+  let ind := .access inds (.var ctr)
   { skip := fun i r ↦
     .branch r
-      (.store (.local ctr) (.int_add $! ![.var .int ctr, .to _ _ $! ![ind <= i]]))
-      (.store (.local ctr) (.int_add $! ![.var .int ctr, .to _ _ $! ![ind << i]]))
+      (.store (.local ctr) (.int_add $! ![.var ctr, .to _ _ $! ![ind <= i]]))
+      (.store (.local ctr) (.int_add $! ![.var ctr, .to _ _ $! ![ind << i]]))
     ready := .true $! ![]
-    valid := .lt $! ![E.var i ctr, E.var i size]
+    valid := .lt $! ![ctr.expr, size.expr]
     index := ind
   }
   --value := .var .int ctr
 --| level (σ : Type) (i : A) (is : List A) (l : Level A i) (f : σ → IStream A σ is) : IStream A σ (i :: is)
 
 inductive Stream {A : Type} : List A → A → Type
+| scalar {i : A} (e : E A (.k i)) : Stream [] i
 | level {i v : A} {is : List A} (l : Level i) (val : (Stream is v)) : Stream (i :: is) v
 | seq {is : List A} (a b : Stream is v) : Stream is v
 | fun {i : A} (f : E A i → Stream is v) : Stream (i :: is) v -- todo, make first order (fix partial)
-| scalar {i : A} (e : E A (.k i)) : Stream [] i
-
+| contraction {is : List A} : Stream (_ :: is) v → Stream is v
 
 infixr:26 " →ₛ " => Stream
-#check [] →ₛ i
 
-instance is0 : Inhabited (Stream [] v) where default := .scalar 0
-instance iss [Inhabited (Stream is v)] : Inhabited (Stream (i :: is) v) where default := .fun fun _ ↦ default
+def Stream.default (is) : Stream is v :=
+match is with
+| [] => .scalar 0
+| (_ :: is) => .fun fun _ ↦ Stream.default is
+
+instance : Inhabited (Stream is v) where default := Stream.default is
 
 namespace Stream
 
-partial def mul {is : List A} {v : A} : is →ₛ v → is →ₛ v → is →ₛ v
-| level l₁ v₁, level l₂ v₂ => level (l₁.mul l₂) $ v₁.mul v₂
+-- "LVS" = L-value stream
 
+abbrev LVSLevel (i : A) := (E A .int → P A) → E A i → P A × E A .int
+inductive LVS : List A → A → Type
+| scalar {v : A} (init : P A) (val : LVal A (.k v)) : LVS [] v
+| level  {i : A} (init : P A) (push_do : E A i → P A) (push_val : E A i → LVS is v)  : LVS (i :: is) v
+
+def LVS.init {is : List A} : LVS is v → P A
+| scalar init _=> init
+| level init _ _ => init
+
+section
+def VarLVS (is : List A) (v : A) : Type := E A .int → LVS is v
+
+variable {is : List A} {i : A}
+
+def composeLValues (level : E A .int → LVSLevel i × P A) : VarLVS is v → VarLVS (i :: is) v :=
+fun val loc ↦
+  let ⟨ l, init ⟩  := level loc
+  let val_init i   := val i |>.init
+  let push_do ind  :=     (l val_init ind).1
+  let push_val ind := val (l val_init ind).2
+  .level init push_do push_val
+
+def sparseLVSLevel_aux (ind_array : Var A i) (lower upper : LVal A .int)
+    : LVSLevel i := fun init ind ↦
+  let loc   := upper.expr - 1
+  let current := E.access ind_array loc
+  let prog := P.if1 (.or $! ![.eq $! ![lower.expr, upper.expr], ind != current]) (upper.incr;; init loc);;
+                P.store (.mem ind_array loc) ind
+  (prog, loc)
+
+def sparseLVSLevel (i : A) (ind_array : Var A i) (arr : Var A .int)
+    : E A .int → LVSLevel i × P A :=
+  let init ind := P.store (.mem arr (ind+1)) (.access arr ind)
+  fun ind ↦ (sparseLVSLevel_aux ind_array (.mem arr ind) (.mem arr (ind+1)), init ind)
+
+def valueScalar (arr : Var A (.k i)) : E A .int → LVS [] i := fun ind ↦ .scalar .skip (.mem arr ind)
+
+#check composeLValues
+#check sparseLVSLevel
+variable (i j : A)
+#check composeLValues (sparseLVSLevel i "ind0" "pos0") $
+       composeLValues (sparseLVSLevel j "ind0" "pos0") $
+       (valueScalar "values")
+
+-- todo: make dense lvslevel
+
+end
+
+#check List.Mem
+#check Finset.mem_erase
+variable [BEq A]
+
+def contract : ∀ {is} (here : is.Here i), Stream is v → Stream (is.eraseHere here) v
+| _, h, .contraction e => .contraction (e.contract (.tail _ h))
+| _, .head _, .fun .. => panic! "cannot contract functional stream"
+| _, .tail _ h', .fun f => .fun fun x ↦ (f x).contract h'
+| _, h, seq a b => .seq (a.contract h) (b.contract h)
+| _, .head _, s@(level ..) => .contraction s
+| _, .tail _ h, level l v => level l (v.contract h)
+
+def expand : ∀ {is} (here : is.Here i), Stream is v → Stream (is.eraseHere here) v
+| _, h, .contraction e => .contraction (e.contract (.tail _ h))
+| _, .head _, .fun .. => panic! "cannot contract functional stream"
+| _, .tail _ h', .fun f => .fun fun x ↦ (f x).contract h'
+| _, h, seq a b => .seq (a.contract h) (b.contract h)
+| _, .head _, s@(level ..) => .contraction s
+| _, .tail _ h, level l v => level l (v.contract h)
+
+def contract' (i : A) [h : List.Find i is] : Stream is v → Stream (is.eraseHere h.here) v
+| s => s.contract List.Find.here
+
+
+def compile : ∀ {is : List A}, LVS is v → is →ₛ v → P A
+| _, _, .fun _ => panic! "cannot generate finite loop for functional stream"
+| _, l, seq a b => a.compile l ;; b.compile l
+| _, .scalar _ l, scalar r => .store l (.add $! ![l.expr, r])
+| _, l, contraction r => compile (.level .skip (fun _ ↦ .skip) (fun _ ↦ l)) r
+| i :: _, .level _ push l', .level r r' => let ready : Var A .bool := "ready"; let index : Var A i := "index"
+    .while r.valid $
+      .let ready r.ready $
+      .let index r.index $
+      (.if1 ready.expr (push index.expr;; compile (l' index.expr) r'));;
+      r.skip index.expr ready.expr
+
+-- | _, l, .memo p s => p ;; compile l s
+--| i, .level _ push l', @Stream.level _ _ _ _ r r' => let ready : Var A .bool := "ready"; let index : Var A i := "index"
+
+partial def mul {is : List A} {v : A} : is →ₛ v → is →ₛ v → is →ₛ v
 | l, seq a b => seq (l.mul a) (l.mul b)
 | seq a b, l => seq (a.mul l) (b.mul l)
 
@@ -216,37 +342,106 @@ partial def mul {is : List A} {v : A} : is →ₛ v → is →ₛ v → is →�
 | .fun f, .level l v => .level l ((f l.index).mul v)
 | .level l v, .fun f => .level l ((f l.index).mul v)
 
+| level l₁ v₁, level l₂ v₂ => level (l₁.mul l₂) $ v₁.mul v₂
+
+| contraction l, r => sorry -- need fresh names, stream for accumulation
+| l, contraction r => sorry
+
 | .scalar e₁, .scalar e₂ => .scalar (.mul $! ![e₁, e₂])
---termination_by _ x y => sizeOf (x, y)
+-- | .memo p₁ s₁, .memo p₂ s₂ =>  .memo (p₁ ;; p₂) (s₁.mul s₂)
+
+--termination_by _ x y => sizeOf (x, y) -- try just (x, y)
 --decreasing_by
 --  try decreasing_tactic <;>
 --  (simp [sizeOf]; sorry)
 
-inductive LValueStream {A : Type} : List A → Type
-| scalar (val : LVal A) : LValueStream []
-| level {i : A} (push : E A i → P A) (val : LValueStream is) : LValueStream (i :: is)
+variable [LinearOrder A]
 
-def compile {is : List A} : LValueStream is → Stream is v → P A
-| _, .fun _ => panic! "cannot generate finite loop for functional stream"
-| l, seq a b => a.compile l ;; b.compile l
-| .scalar l, scalar r => .store l (.add $! ![l.expr, r])
-| .level push l', .level r r' =>
-    let ready : Var := "ready"
-    let index : Var := "index"
-    .while r.valid $
-      .let ready r.ready $
-      .let index r.index $
-      (.if1 (ready.expr _)
-        (push r.index;; compile l' r'))
-      ;; r.skip (index.expr _) (ready.expr _)
+-- TODO try insertHere instead?
+def insert : A → List A → List A
+| j, []  => [j]
+| j, i :: is => if j = i then i :: is else if j < i then j :: i :: is else i :: is.insert j
+
+#check ne_of_lt
+@[simp] theorem insert_lt (h : j < i) : insert j (i :: is) = j :: i :: is := by
+  dsimp [insert];
+  split; rename_i h'
+  cases ne_of_lt h h'; rfl
+
+@[simp] theorem insert_gt (h : i < j) : insert j (i :: is) = i :: insert j is := by
+  dsimp [insert];
+  split <;> rename_i h'
+  . cases ne_of_lt h h'.symm;
+  . split; rename_i h''
+    cases not_lt_of_gt h h''
+    sorry
+    sorry
+
+
+@[simp] theorem insert_lt (h : j < i) : insert j (i :: is) = j :: i :: is := by
+  dsimp [insert]; split; contradiction; rfl; contradiction
+
+-- need nested match in order for simp lemmas to work below
+def merge : List A → List A → List A
+| [], x => x
+| x :: xs, ys =>
+  match ys with
+    | [] => x :: xs
+    | y :: ys => if x = y then x :: merge xs ys else
+      if x < y then x :: merge xs (y :: ys) else y :: merge (x :: xs) ys
+termination_by _ x y => (x, y)
+
+#print merge._unary
+#eval merge [1,3] [0,2]
+
+section merge
+@[simp] theorem nil_merge (x : List A) : merge [] x = x := by rw [merge]
+@[simp] theorem merge_nil (x : List A) : merge x [] = x := by cases x <;> rw [merge] -- can't just `rw [merge]`
+end merge
+
+def expand_lt (j : A) (h : j < i) : ∀ {is}, Stream (i :: is) v → Stream (insert j (i :: is)) v
+|_, s => by rw [insert_lt h]; exact .fun fun _ ↦ s
+def expand_eq (j : A) (h : j = i) : Stream (i :: is) v → Stream (insert j (i :: is)) v
+| s => by dsimp [insert]; simpa [h] using s
+def expand_gt (j : A) (h : i < j) : ∀ {is}, Stream (i :: is) v → Stream (insert j (i :: is)) v
+| _, .contraction e => .contraction (e.expand (.tail _ h))
+| _,  .fun .. => panic! "cannot contract functional stream"
+| _, .fun f => .fun fun x ↦ (f x).contract h'
+| _, seq a b => .seq (a.contract h) (b.contract h)
+| _, s@(level ..) => .contraction s
+| _, level l v => level l (v.contract h)
+
+example : ¬ j < i → i ≤ j := by simp?
+
+def expand (j : A) : ∀ {is}, is →ₛ v → insert j is →ₛ v
+| [], s => .fun fun _ ↦ s
+| i :: _, s => lt_by_cases j i (fun h ↦ expand_lt j h s) (fun h ↦ expand_eq j h s) fun h ↦
+  match s with
+  | .fun f => .fun fun i ↦ (f i).expand j
+  expand_gt j h s
+
+def expand : [] →ₛv →  is →ₛv := sorry
+
+--def mul' [LinearOrder A] : (is : List A) → (js : List A) → is →ₛ v → js →ₛ v → ((merge is js →ₛ v) × ((merge is js →ₛ v)))
+--| [], x, s, t => by rw [nil_merge]; exact (s.expand, t)
+--| x, [], s, t => by rw [merge_nil]; exact (s, t.expand)
+--| x :: xs, y :: ys, s, t => if x = y
+--  then sorry else if true
+--  then x :: merge xs (y :: ys) else y :: merge (x :: xs) ys
+
+variable (i j k : A)
+#check (contract' i $ default [i, j])
+#check let a  : [j] →ₛ i := (contract' i (default [i, j])); a
 
 end Stream
 end Etch
 
 /- todo
   define contraction, expansion, fast addition for new stream type
-  lvalstream
+    [X] mapped contraction
+    [ ] mapped expansion, mul
+    [ ] (lval, rval) pairs. memo? finish compile.
   test output
 
-  refactor lval
+  [X] refactor lval
 -/
